Introducing more failure variants

src/Testing/PrintRISCVTagSimpleEager.v
@@ -13,8 +13,8 @@ Require Import coqutil.Map.Z_keyed_SortedListMap.
 Require Import coqutil.Map.Interface.
 Require Import Coq.Lists.List. Import ListNotations.
 
-Module PrintRISCVTagSimpleEager : Printing RISCVObs TPEagerObs DLObs TSS.
-  Module MPC := TestMPC RISCVObs TPEagerObs DLObs TSS.
+Module PrintRISCVEager : Printing RISCVObs TPEager DLObs TSS.
+  Module MPC := TestMPC RISCVObs TPEager DLObs TSS.
   Import MPC.
 
   Definition printObsType (o:ObsType) := "".
@@ -156,4 +156,439 @@ Module PrintRISCVTagSimpleEager : Printing RISCVObs TPEagerObs DLObs TSS.
   Instance ShowMP : Show (MachineState * PolicyState * CodeMap_Impl):=
     {| show := fun '(m,p,cm) => printMachine m p cm (initCtx defLayoutInfo) |}.
 
-End PrintRISCVTagSimpleEager.
+End PrintRISCVEager.
+
+Module PrintRISCVEagerNLC : Printing RISCVObs TPEagerNLC DLObs TSS.
+  Module MPC := TestMPC RISCVObs TPEagerNLC DLObs TSS.
+  Import MPC.
+
+  Definition printObsType (o:ObsType) := "".
+  Instance ShowObsType : Show ObsType :=
+    {| show o := printObsType o |}.
+  Derive Show for Observation.
+
+  Definition printPC (m : MachineState) (p : PolicyState) :=
+  (show (projw m PC) ++ " @ " ++ show (pctags p))%string.
+
+  Definition printPCs (m n : MachineState) (p : PolicyState) :=
+    let val1 := projw m PC in
+    let val2 := projw n PC in
+    ((if Z.eqb val1 val2 then
+        show val1
+      else (show val1 ++ "/" ++ show val2))
+       ++ " @ " ++ show (pctags p))%string.
+
+  Instance ShowCodeAnnotation : Show CodeAnnotation :=
+    {| show ca :=
+         match ca with
+         | call => "call"
+         | yield => "yield"
+         | scall _ => "scall"
+         | normal => "normal"
+         | _  => "ret"
+         end |}.
+
+  Derive Show for StackDomain.
+  
+  Definition printComponent (k : Component)
+           (m : MachineState) (p : PolicyState)
+           (cm : CodeMap_Impl) (c : CtxState)
+           (i : LayoutInfo) :=
+  let val := proj m k in
+  let tag := pproj p k in
+  match k with
+  | Mem a =>
+    (* Check if in instruction memory *)
+    if andb (Z.leb (instLo i) a) (Z.leb a (instHi i))
+    then
+      match decode RV32I val with
+      | IInstruction inst =>
+        ("[" ++ show a ++ "] : " ++ show inst ++ " @ " ++ show tag ++ " < " ++ show (CodeMap_fromImpl cm a) ++ " > - " ++ show (fst c (Mem a)))%string
+      | _ => (show val ++ " <not-inst>")%string
+      end
+    else
+      ("[" ++ show a ++ "]" ++ show val ++ " @" ++ show tag ++ " < " ++ show (CodeMap_fromImpl cm a) ++ " > - " ++ show (fst c (Mem a)))%string
+  | Reg r => 
+    ("r" ++ show r ++ " : " ++ show val ++ " @ " ++ show tag) %string
+  | PC => ("PC: " ++ printPC m p ++ " - " ++
+      match decode RV32I (proj m (Mem val)) with
+      | IInstruction inst =>
+        (show inst)
+      | _ => (show val ++ " <not-inst>")%string
+      end)%string
+  end.
+
+  Definition listify1 {A} (m : Zkeyed_map A)
+    : list (Z * A) :=
+    List.rev (map.fold (fun acc z v => (z,v) :: acc) nil m).
+  
+  Fixpoint combine_match {A B} `{Show A} `{Show B}
+           (l1 : list (Z * A)) (l2 : list (Z * B))
+    : list (Z * A * B) :=
+    match l1, l2 with
+    | (z1,a)::l1',(z2,b)::l2' =>
+      if Z.eqb z1 z2 then
+        (z1, a, b) :: combine_match l1' l2'
+      else combine_match l1' l2' (*exception ("combine_match - not_eq " ++ (show (l1, l2))%string)*)
+    | nil, nil => nil
+    | _, _ => nil (*exception ("combine_match: " ++ (show (l1,l2)))%string*)
+    end.
+
+  Definition listify2 {A B} `{Show A} `{Show B}
+             (m1 : Zkeyed_map A)
+             (m2 : Zkeyed_map B) : list (Z * A * B) :=
+    combine_match (listify1 m1) (listify1 m2).
+
+  Definition printGPRs (m : MachineState) (p : PolicyState) :=
+    List.fold_left (fun acc '(rID, rVal, rTag) =>
+                      show rID ++ " : " ++ show rVal ++ " @ " ++ show rTag ++ nl ++ acc)%string 
+                   (listify2 (getRegs m) (regtags p)) "".
+
+  Definition listify1_word mem := 
+  List.rev
+    (map.fold
+       (fun acc k v =>
+          (* Keep mod 4 *)
+          if Z.eqb (snd (Z.div_eucl (word.unsigned k) 4)) 0
+          then
+            let val := 
+                match loadWord mem k with
+                | Some w32 => LittleEndian.combine _ w32
+                | _ => 42424242
+                end in
+            (word.unsigned k,val) :: acc
+          else acc) nil mem).
+
+  Definition printMem (m : MachineState) (p : PolicyState) (cm : CodeMap_Impl) (c : CtxState) (i : LayoutInfo) :=
+    let mem := getMem m in
+    let tags := memtags p in
+    let mts := combine_match (listify1_word mem) (listify1 tags) in
+    List.fold_left
+      (fun s '(k,val,t) =>
+         let printed :=
+             if andb (Z.leb (instLo i) k)
+                     (Z.leb k (instHi i))
+             then
+               match decode RV32I val with
+               | IInstruction inst =>
+                 (show inst ++ " @ " ++ show t ++ " < " ++ show (CodeMap_fromImpl cm k) ++ " > - " ++ show (fst c (Mem k)))%string
+               | _ => (show val ++ " <not-inst>")%string
+               end
+             else
+               (show val ++ " @" ++ show t ++ " < " ++ show (CodeMap_fromImpl cm k) ++ " > - " ++ show (fst c (Mem k)))%string in
+         if andb (Z.eqb val 0) (seq.nilp t) then
+           s
+         else 
+           (show k ++ " : " ++ printed ++ nl ++ s)%string
+      ) mts "".
+
+  
+  Definition printMachine (m : MachineState) (p : PolicyState) cm c :=
+    (
+      "PC:" ++  
+      printPC m p ++ nl ++
+      "Registers:" ++ nl ++
+      printGPRs m p ++ nl ++
+      "Memory: " ++ nl ++
+      printMem m p cm c defLayoutInfo ++ nl
+    )%string.
+
+  Derive Show for Component.
+
+  Instance ShowValue : Show Value :=
+    {| show v := show v |}.
+
+  Instance ShowMP : Show (MachineState * PolicyState * CodeMap_Impl):=
+    {| show := fun '(m,p,cm) => printMachine m p cm (initCtx defLayoutInfo) |}.
+
+End PrintRISCVEagerNLC.
+
+Module PrintRISCVEagerNSC : Printing RISCVObs TPEagerNSC DLObs TSS.
+  Module MPC := TestMPC RISCVObs TPEagerNSC DLObs TSS.
+  Import MPC.
+
+  Definition printObsType (o:ObsType) := "".
+  Instance ShowObsType : Show ObsType :=
+    {| show o := printObsType o |}.
+  Derive Show for Observation.
+
+  Definition printPC (m : MachineState) (p : PolicyState) :=
+  (show (projw m PC) ++ " @ " ++ show (pctags p))%string.
+
+  Definition printPCs (m n : MachineState) (p : PolicyState) :=
+    let val1 := projw m PC in
+    let val2 := projw n PC in
+    ((if Z.eqb val1 val2 then
+        show val1
+      else (show val1 ++ "/" ++ show val2))
+       ++ " @ " ++ show (pctags p))%string.
+
+  Instance ShowCodeAnnotation : Show CodeAnnotation :=
+    {| show ca :=
+         match ca with
+         | call => "call"
+         | yield => "yield"
+         | scall _ => "scall"
+         | normal => "normal"
+         | _  => "ret"
+         end |}.
+
+  Derive Show for StackDomain.
+  
+  Definition printComponent (k : Component)
+           (m : MachineState) (p : PolicyState)
+           (cm : CodeMap_Impl) (c : CtxState)
+           (i : LayoutInfo) :=
+  let val := proj m k in
+  let tag := pproj p k in
+  match k with
+  | Mem a =>
+    (* Check if in instruction memory *)
+    if andb (Z.leb (instLo i) a) (Z.leb a (instHi i))
+    then
+      match decode RV32I val with
+      | IInstruction inst =>
+        ("[" ++ show a ++ "] : " ++ show inst ++ " @ " ++ show tag ++ " < " ++ show (CodeMap_fromImpl cm a) ++ " > - " ++ show (fst c (Mem a)))%string
+      | _ => (show val ++ " <not-inst>")%string
+      end
+    else
+      ("[" ++ show a ++ "]" ++ show val ++ " @" ++ show tag ++ " < " ++ show (CodeMap_fromImpl cm a) ++ " > - " ++ show (fst c (Mem a)))%string
+  | Reg r => 
+    ("r" ++ show r ++ " : " ++ show val ++ " @ " ++ show tag) %string
+  | PC => ("PC: " ++ printPC m p ++ " - " ++
+      match decode RV32I (proj m (Mem val)) with
+      | IInstruction inst =>
+        (show inst)
+      | _ => (show val ++ " <not-inst>")%string
+      end)%string
+  end.
+
+  Definition listify1 {A} (m : Zkeyed_map A)
+    : list (Z * A) :=
+    List.rev (map.fold (fun acc z v => (z,v) :: acc) nil m).
+  
+  Fixpoint combine_match {A B} `{Show A} `{Show B}
+           (l1 : list (Z * A)) (l2 : list (Z * B))
+    : list (Z * A * B) :=
+    match l1, l2 with
+    | (z1,a)::l1',(z2,b)::l2' =>
+      if Z.eqb z1 z2 then
+        (z1, a, b) :: combine_match l1' l2'
+      else combine_match l1' l2' (*exception ("combine_match - not_eq " ++ (show (l1, l2))%string)*)
+    | nil, nil => nil
+    | _, _ => nil (*exception ("combine_match: " ++ (show (l1,l2)))%string*)
+    end.
+
+  Definition listify2 {A B} `{Show A} `{Show B}
+             (m1 : Zkeyed_map A)
+             (m2 : Zkeyed_map B) : list (Z * A * B) :=
+    combine_match (listify1 m1) (listify1 m2).
+
+  Definition printGPRs (m : MachineState) (p : PolicyState) :=
+    List.fold_left (fun acc '(rID, rVal, rTag) =>
+                      show rID ++ " : " ++ show rVal ++ " @ " ++ show rTag ++ nl ++ acc)%string 
+                   (listify2 (getRegs m) (regtags p)) "".
+
+  Definition listify1_word mem := 
+  List.rev
+    (map.fold
+       (fun acc k v =>
+          (* Keep mod 4 *)
+          if Z.eqb (snd (Z.div_eucl (word.unsigned k) 4)) 0
+          then
+            let val := 
+                match loadWord mem k with
+                | Some w32 => LittleEndian.combine _ w32
+                | _ => 42424242
+                end in
+            (word.unsigned k,val) :: acc
+          else acc) nil mem).
+
+  Definition printMem (m : MachineState) (p : PolicyState) (cm : CodeMap_Impl) (c : CtxState) (i : LayoutInfo) :=
+    let mem := getMem m in
+    let tags := memtags p in
+    let mts := combine_match (listify1_word mem) (listify1 tags) in
+    List.fold_left
+      (fun s '(k,val,t) =>
+         let printed :=
+             if andb (Z.leb (instLo i) k)
+                     (Z.leb k (instHi i))
+             then
+               match decode RV32I val with
+               | IInstruction inst =>
+                 (show inst ++ " @ " ++ show t ++ " < " ++ show (CodeMap_fromImpl cm k) ++ " > - " ++ show (fst c (Mem k)))%string
+               | _ => (show val ++ " <not-inst>")%string
+               end
+             else
+               (show val ++ " @" ++ show t ++ " < " ++ show (CodeMap_fromImpl cm k) ++ " > - " ++ show (fst c (Mem k)))%string in
+         if andb (Z.eqb val 0) (seq.nilp t) then
+           s
+         else 
+           (show k ++ " : " ++ printed ++ nl ++ s)%string
+      ) mts "".
+
+  
+  Definition printMachine (m : MachineState) (p : PolicyState) cm c :=
+    (
+      "PC:" ++  
+      printPC m p ++ nl ++
+      "Registers:" ++ nl ++
+      printGPRs m p ++ nl ++
+      "Memory: " ++ nl ++
+      printMem m p cm c defLayoutInfo ++ nl
+    )%string.
+
+  Derive Show for Component.
+
+  Instance ShowValue : Show Value :=
+    {| show v := show v |}.
+
+  Instance ShowMP : Show (MachineState * PolicyState * CodeMap_Impl):=
+    {| show := fun '(m,p,cm) => printMachine m p cm (initCtx defLayoutInfo) |}.
+
+End PrintRISCVEagerNSC.
+
+Module PrintRISCVEagerNI : Printing RISCVObs TPEagerNI DLObs TSS.
+  Module MPC := TestMPC RISCVObs TPEagerNI DLObs TSS.
+  Import MPC.
+
+  Definition printObsType (o:ObsType) := "".
+  Instance ShowObsType : Show ObsType :=
+    {| show o := printObsType o |}.
+  Derive Show for Observation.
+
+  Definition printPC (m : MachineState) (p : PolicyState) :=
+  (show (projw m PC) ++ " @ " ++ show (pctags p))%string.
+
+  Definition printPCs (m n : MachineState) (p : PolicyState) :=
+    let val1 := projw m PC in
+    let val2 := projw n PC in
+    ((if Z.eqb val1 val2 then
+        show val1
+      else (show val1 ++ "/" ++ show val2))
+       ++ " @ " ++ show (pctags p))%string.
+
+  Instance ShowCodeAnnotation : Show CodeAnnotation :=
+    {| show ca :=
+         match ca with
+         | call => "call"
+         | yield => "yield"
+         | scall _ => "scall"
+         | normal => "normal"
+         | _  => "ret"
+         end |}.
+
+  Derive Show for StackDomain.
+  
+  Definition printComponent (k : Component)
+           (m : MachineState) (p : PolicyState)
+           (cm : CodeMap_Impl) (c : CtxState)
+           (i : LayoutInfo) :=
+  let val := proj m k in
+  let tag := pproj p k in
+  match k with
+  | Mem a =>
+    (* Check if in instruction memory *)
+    if andb (Z.leb (instLo i) a) (Z.leb a (instHi i))
+    then
+      match decode RV32I val with
+      | IInstruction inst =>
+        ("[" ++ show a ++ "] : " ++ show inst ++ " @ " ++ show tag ++ " < " ++ show (CodeMap_fromImpl cm a) ++ " > - " ++ show (fst c (Mem a)))%string
+      | _ => (show val ++ " <not-inst>")%string
+      end
+    else
+      ("[" ++ show a ++ "]" ++ show val ++ " @" ++ show tag ++ " < " ++ show (CodeMap_fromImpl cm a) ++ " > - " ++ show (fst c (Mem a)))%string
+  | Reg r => 
+    ("r" ++ show r ++ " : " ++ show val ++ " @ " ++ show tag) %string
+  | PC => ("PC: " ++ printPC m p ++ " - " ++
+      match decode RV32I (proj m (Mem val)) with
+      | IInstruction inst =>
+        (show inst)
+      | _ => (show val ++ " <not-inst>")%string
+      end)%string
+  end.
+
+  Definition listify1 {A} (m : Zkeyed_map A)
+    : list (Z * A) :=
+    List.rev (map.fold (fun acc z v => (z,v) :: acc) nil m).
+  
+  Fixpoint combine_match {A B} `{Show A} `{Show B}
+           (l1 : list (Z * A)) (l2 : list (Z * B))
+    : list (Z * A * B) :=
+    match l1, l2 with
+    | (z1,a)::l1',(z2,b)::l2' =>
+      if Z.eqb z1 z2 then
+        (z1, a, b) :: combine_match l1' l2'
+      else combine_match l1' l2' (*exception ("combine_match - not_eq " ++ (show (l1, l2))%string)*)
+    | nil, nil => nil
+    | _, _ => nil (*exception ("combine_match: " ++ (show (l1,l2)))%string*)
+    end.
+
+  Definition listify2 {A B} `{Show A} `{Show B}
+             (m1 : Zkeyed_map A)
+             (m2 : Zkeyed_map B) : list (Z * A * B) :=
+    combine_match (listify1 m1) (listify1 m2).
+
+  Definition printGPRs (m : MachineState) (p : PolicyState) :=
+    List.fold_left (fun acc '(rID, rVal, rTag) =>
+                      show rID ++ " : " ++ show rVal ++ " @ " ++ show rTag ++ nl ++ acc)%string 
+                   (listify2 (getRegs m) (regtags p)) "".
+
+  Definition listify1_word mem := 
+  List.rev
+    (map.fold
+       (fun acc k v =>
+          (* Keep mod 4 *)
+          if Z.eqb (snd (Z.div_eucl (word.unsigned k) 4)) 0
+          then
+            let val := 
+                match loadWord mem k with
+                | Some w32 => LittleEndian.combine _ w32
+                | _ => 42424242
+                end in
+            (word.unsigned k,val) :: acc
+          else acc) nil mem).
+
+  Definition printMem (m : MachineState) (p : PolicyState) (cm : CodeMap_Impl) (c : CtxState) (i : LayoutInfo) :=
+    let mem := getMem m in
+    let tags := memtags p in
+    let mts := combine_match (listify1_word mem) (listify1 tags) in
+    List.fold_left
+      (fun s '(k,val,t) =>
+         let printed :=
+             if andb (Z.leb (instLo i) k)
+                     (Z.leb k (instHi i))
+             then
+               match decode RV32I val with
+               | IInstruction inst =>
+                 (show inst ++ " @ " ++ show t ++ " < " ++ show (CodeMap_fromImpl cm k) ++ " > - " ++ show (fst c (Mem k)))%string
+               | _ => (show val ++ " <not-inst>")%string
+               end
+             else
+               (show val ++ " @" ++ show t ++ " < " ++ show (CodeMap_fromImpl cm k) ++ " > - " ++ show (fst c (Mem k)))%string in
+         if andb (Z.eqb val 0) (seq.nilp t) then
+           s
+         else 
+           (show k ++ " : " ++ printed ++ nl ++ s)%string
+      ) mts "".
+
+  
+  Definition printMachine (m : MachineState) (p : PolicyState) cm c :=
+    (
+      "PC:" ++  
+      printPC m p ++ nl ++
+      "Registers:" ++ nl ++
+      printGPRs m p ++ nl ++
+      "Memory: " ++ nl ++
+      printMem m p cm c defLayoutInfo ++ nl
+    )%string.
+
+  Derive Show for Component.
+
+  Instance ShowValue : Show Value :=
+    {| show v := show v |}.
+
+  Instance ShowMP : Show (MachineState * PolicyState * CodeMap_Impl):=
+    {| show := fun '(m,p,cm) => printMachine m p cm (initCtx defLayoutInfo) |}.
+
+End PrintRISCVEagerNI.
